more

Weidenbach_Book/IsaSAT/Heaps_Abs.thy
@@ -31,6 +31,7 @@ begin
     definition mop_prio_change_weight where
       "mop_prio_change_weight \<equiv>  (\<lambda>v \<omega> (\<A>, b, w). doN {
         ASSERT (v \<in># \<A>);
+        ASSERT (v \<in># b \<longrightarrow> le \<omega> (w v));
         RETURN (\<A>, b, w(v := \<omega>))
      })"
 
@@ -40,9 +41,15 @@ begin
         RETURN (\<A>, add_mset v b, w(v := \<omega>))
      })"
 
+    definition mop_prio_is_in where
+      \<open>mop_prio_is_in = (\<lambda>v (\<A>, b, w). do {
+      ASSERT (v \<in># \<A>);
+      RETURN (v \<in>#b)
+      })\<close>
     definition mop_prio_insert_maybe where
       "mop_prio_insert_maybe \<equiv>  (\<lambda>v \<omega> (bw). doN {
-        if v \<notin># fst (snd bw) then mop_prio_insert v \<omega> (bw)
+        b \<leftarrow> mop_prio_is_in v bw;
+        if \<not>b then mop_prio_insert v \<omega> (bw)
         else mop_prio_change_weight v \<omega> (bw)
      })"
 
@@ -54,7 +61,8 @@ begin
 
     definition mop_prio_insert_unchanged where
       "mop_prio_insert_unchanged =  (\<lambda>v (bw). doN {
-        if v \<notin># fst (snd bw) then mop_prio_insert_raw_unchanged v (bw)
+        b \<leftarrow> mop_prio_is_in v bw;
+        if \<not>b then mop_prio_insert_raw_unchanged v (bw)
         else RETURN bw
      })"
 
@@ -68,9 +76,9 @@ begin
      })"
 
     definition mop_prio_pop_min where
-      "mop_prio_pop_min = (\<lambda>(\<A>, b, w). doN {ASSERT (b\<noteq>{#});
-      v \<leftarrow> mop_prio_peek_min (\<A>, b, w);
-      bw \<leftarrow> mop_prio_del v (\<A>, b, w);
+      "mop_prio_pop_min = (\<lambda>\<A>bw. doN {
+      v \<leftarrow> mop_prio_peek_min \<A>bw;
+      bw \<leftarrow> mop_prio_del v \<A>bw;
       RETURN (v, bw)
       })"
 
